theories/CombinatoryLogic/Plotkin.v
@@ -12,12 +12,6 @@ Require Import Relations.
 From Undecidability Require Import CombinatoryLogic.Krivine.
 
 Require Import ssreflect ssrbool ssrfun.
-   
-(* left-most outer-most call-by-name *)
-Inductive step : term -> term -> Prop :=
-  | stepLam s t    : step (app (lam s) t) (subst s 0 t)
-  | stepApp s s' t : step s s' -> step (app s t) (app s' t).
-
 
 Fixpoint cbv_cbn (t : term) : term :=
   match t with
@@ -30,15 +24,37 @@ Definition Psi (t : term) :=
   match t with
   | var n => var n
   | app s t => app s t
-  | lam s => ren S (lam (cbv_cbn s))
+  | lam s => lam (cbv_cbn s)
   end.
 
+(*
 Lemma subst_ren s k t : subst (ren S s) (S k) t = ren S (subst s k t).
 Proof. Admitted. (* needs closedness *)
+*)
 
-Lemma lemma_6_1 M N k : 
-  subst (cbv_cbn M) k (Psi (lam N)) = cbv_cbn (subst M k (lam N)).
+Lemma lemma_6_1 s k t : closed (lam t) ->
+  cbv_cbn (L.subst s k (lam t)) = L.subst (cbv_cbn s) k (Psi (lam t)).
 Proof.
+  move=> Ht. elim: s k.
+  - move=> n k /=. case: (Nat.eqb n k); last done.
+    move=> /=. congr lam. congr app. congr lam. admit. (* use closedness *)
+  - move=> s1 IH1 s2 IH2 k /=. rewrite IH1 IH2 /=.
+    congr lam. congr app.
+    + admit.
+    + congr lam. congr app. admit.
+  - move=> s IH k /=. rewrite IH /=.
+    congr lam. congr app. congr lam.
+    admit.
+Admitted.
+
+(*
+Lemma lemma_6_1 M N :
+  subst (scons (Psi (lam N)) var) (cbv_cbn M) = cbv_cbn (subst (scons (lam N) var) M).
+Proof.
+  (* maybe point subst is better ?  *)
+Admitted.
+*)
+(*
   elim: M k N.
   - move=> /= n k N. case: (Nat.eqb n k).
     + done.
@@ -51,6 +67,7 @@ Proof.
     congr lam. congr app. congr lam.
     cbn.
 Admitted.
+*)
 
 Definition on_app {X : Type} (s : term) (x : X) (g : term -> term -> X) : X :=
   match s with
@@ -58,7 +75,25 @@ Definition on_app {X : Type} (s : term) (x : X) (g : term -> term -> X) : X :=
   | _ => x
   end.
 
+Definition is_app (s: term) : bool :=
+  if s is app _ _ then true else false.
+
+Fixpoint colon (M : term) (u : term) : term :=
+  match M with
+  | var _ => app u (Psi M)
+  | lam _ => app u (Psi M)
+  | app s t =>
+      if is_app s then
+        colon s (lam (app (ren S (cbv_cbn t)) (lam (app (app (var 1) (var 0)) (ren S (ren S u))))))
+      else
+        if is_app t then
+          colon t (lam (app (app (ren S (Psi s)) (var 0)) (ren S u)))
+        else
+          app (app (Psi s) (Psi t)) u
+  end.
+
 (* plotkins M : K *)
+(*
 Fixpoint colon (M : term) (u : term) : term :=
   on_app M (
     app u (Psi M)
@@ -68,36 +103,169 @@ Fixpoint colon (M : term) (u : term) : term :=
         on_app t (
           app (app (Psi s) (Psi t)) u
         ) (
-          fun t1 t2 => app (Psi t) (lam (app (app (app (var 0) (Psi s)) (var 0)) u))
+          fun t1 t2 => colon t (lam (app (app (ren S (Psi s)) (var 0)) (ren S u)))
         )
       ) (
-        fun s1 s2 => colon s (lam (app (cbv_cbn t) (lam (app (app (var 1) (var 0)) u))))
+        fun s1 s2 => colon s (lam (app (ren S (cbv_cbn t)) (lam (app (app (var 1) (var 0)) (ren S (ren S u))))))
       )
   ).
 
+Arguments colon : simpl never.
+*)
 
-Lemma lemma_6_2 s u : closed (lam u) -> halt_cbn [] [] (colon s u) -> halt_cbn [] [] (app (cbv_cbn s) u).
+Lemma colon_var_app n t1 t2 u : colon (app (var n) (app t1 t2)) u = colon (app t1 t2) (lam (app (app (ren S (Psi (var n))) (var 0)) (ren S u))).
+Proof. done. Qed.
+  (*
+Lemma ren_const_ren m xi t : ren (fun=> m) (ren xi t) = ren (fun=> m) t.
+Proof. by rewrite ren_ren_term. Qed.
+*)
+
+(* transforms a goal (A -> B) -> C into goals A and B -> C *)
+Lemma unnest : forall (A B C : Type), A -> (B -> C) -> (A -> B) -> C.
+Proof. auto. Qed.
+
+Arguments cbv_cbn: simpl never.
+
+
+(* drop closedness? 
+Lemma lemma_6_2 s u : halt_cbn [] [] (colon s u) -> halt_cbn [] [] (app (cbv_cbn s) u).
 Proof.
-  move=> Hu. elim: s.
-  - move=> n /=.
+  elim: s u.
+  - move=> n u /=.
     move=> /halt_cbnE H'.
     do ? constructor.
-    apply: (halt_cbn_flatten_iff H').
+    apply: (halt_cbn_flatten_iff H'); by constructor.
+  - move=> [n1|s1 s2|s1] IH1 [n2|t1 t2|t1] IH2 u.
+    + move=> /= /halt_cbnE /halt_cbnE H'.
+      do ? constructor.
+      apply: (halt_cbn_flatten_iff H'); last done.
+      constructor; [|constructor;[|done]] => /=.
+      all: by rewrite ren_ren_term.
+    + move Et: (app t1 t2) IH2 => t IH2 /= H'.
+      rewrite /cbv_cbn -/cbv_cbn /= /funcomp /=.
+      do 8 constructor.
+      do 2 apply: halt_cbn_ren_S.
+      have := IH2 (lam (app (app (Psi (var (S n1))) (var 0)) (ren S u))).
+      apply: unnest.
+      { move: H'. by rewrite -Et. }
+      move=> /halt_cbnE {}H'.
+      apply: (halt_cbn_flatten_iff H'); last done.
+      constructor; last done.
+      move=> /=. rewrite /funcomp /many_subst /=.
+      congr lam. rewrite !simpl_term. congr app.
+      apply: ext_subst_term. by case.
+      + admit.
+      + admit.
+      + admit.
+      + admit.
+      + admit.
+      + admit.
+      + admit.
+  - move=> s IH u /=.
+    rewrite /colon -/colon /cbv_cbn -/cbv_cbn /=.
+    move=> /halt_cbnE H'.
+    do ? constructor.
+    apply: (halt_cbn_flatten_iff H'); last done.
+    constructor; last done.
+    move=> /=. rewrite !simpl_term.
+    congr lam. apply: ext_subst_term. by case.
+Admitted.
+*)
 
-
-Lemma main s t : s ≻ t -> 
-  halt_cbn [] [] (app (cbv_cbn s) (lam (var 0))) -> 
-  halt_cbn [] [] (app (cbv_cbn t) (lam (var 0))).
+Lemma bound_cbv_cbn k t : bound k t -> bound k (cbv_cbn t).
 Proof.
-  elim; clear s t.
-  - move=> s t /=.
-    do 17 (move=> /halt_cbnE).
-    move=> H'.
+  elim: t.
+  - move=> n H. rewrite /cbv_cbn.
+Admitted.
 
-  move=> /eval_iff.
-  elim. elim.
-  { admit. }
+Lemma closed_cbv_cbn t : closed t -> closed (cbv_cbn t).
+Proof. Admitted.
 
-  move=> > []. 
+Lemma closed_lam_cbv_cbn t : closed (lam t) -> closed (lam (cbv_cbn t)).
+Proof. Admitted.
 
-Lemma test :=
+Lemma lemma_6_3 {s t u} : closed s -> s ≻ t -> 
+  halt_cbn [] [] (colon t u) ->
+  halt_cbn [] [] (colon s u).
+Proof.
+  move=> Hs Hst.
+  elim: Hst u Hs; clear s t.
+  - move=> s t u /= /closed_app [Hs Ht].
+    move=> H'. rewrite /colon /=.
+    do 3 constructor.
+    suff : halt_cbn [closure [] u] [] (L.subst (cbv_cbn s) 0 (lam (cbv_cbn t))).
+    { move=> {}H'. apply: (halt_cbn_flatten_iff H'); first by constructor.
+      move: Ht => /closed_lam_cbv_cbn. move: (cbv_cbn s) (lam (cbv_cbn t)) => s' t'.
+      admit. (* doable *) }
+    rewrite -lemma_6_1; first done.
+    admit.
+    (* by move: H' => /lemma_6_2 /halt_cbnE. *)
+  - move=> s t t' ? IH u /closed_app [Hs Ht].
+    move=> H'. rewrite /colon -/colon /=.
+Admitted.
+
+Arguments clos_trans {A} R.
+
+(* induction on size of s *)
+Lemma lemma_6_3' {s t u} : closed s -> s ≻ t ->
+  clos_trans step (colon s u) (colon t u).
+Proof.
+  elim /(measure_rect term_size) : s t u.
+  move=> s + t ++ Hst. case: Hst; clear s t.
+  - move=> s1 s2 IH u /closed_app [Hs1 Hs2].
+    rewrite L_subst_subst; first done.
+
+    admit. (* substitution case *)
+    (*
+    move=> H'. rewrite /colon /=.
+    do 3 constructor.
+    suff : halt_cbn [closure [] u] [] (L.subst (cbv_cbn s) 0 (lam (cbv_cbn t))).
+    { move=> {}H'. apply: (halt_cbn_flatten_iff H'); first by constructor.
+      move: Ht => /closed_lam_cbv_cbn. move: (cbv_cbn s) (lam (cbv_cbn t)) => s' t'.
+      admit. (* doable *) }
+    rewrite -lemma_6_1; first done.
+    by move: H' => /lemma_6_2 /halt_cbnE.*)
+  - move=> s t t' ? IH u /closed_app [Hs Ht].
+    rewrite /colon -/colon /=.
+
+
+Admitted.
+
+(* forward simulation *)
+Lemma main_forward s t : closed s -> L.eval s t -> 
+  halt_cbn [] [] (colon s (lam (var 0))).
+Proof.
+  move=> Hs /eval_iff [] Hst Ht.
+  have H't := closed_star Hst Hs.
+  elim: Hst Ht Hs.
+  { move=> ? [? ->] ?. by do ? constructor. }
+  move=> s1 s2 s3 Hs1s2 Hs2s3 IH Hs3 Hs1.
+  apply: lemma_6_3; [done|eassumption|].
+  apply: IH; [done|].
+  by apply: closed_step; eassumption.
+Qed.
+
+Lemma not_halt_cbn_colon_var n : not (halt_cbn [] [] (colon (var n) (lam (var 0)))).
+Proof.
+  move=> /halt_cbnE /halt_cbnE /halt_cbnE /halt_cbnE /=.
+  by case: n.
+Qed.
+
+Lemma main_backward s :
+  closed s -> clos_refl_trans step (colon s u) (colon (lam t) u) -> 
+  
+  halt_cbn [] [] (colon s (lam (var 0))) -> exists t, L.eval s t.
+Proof.
+
+Lemma main_backward s :
+  closed s -> halt_cbn [] [] (colon s (lam (var 0))) -> exists t, L.eval s t.
+Proof.
+  have := Seval.stepf_spec s.
+  case: (Seval.stepf s) => [|s' ?].
+  - admit.
+  - move=> /(_ s') /iffLR /(_ (or_introl erefl)).
+    move=> /lemma_6_3 /[apply]. /[apply].
+    have /[apply] := lemma_6_3 Hs Hss'.
+  Print or.
+
+Check Seval.stepf.
